More changes required by the change to REDUCE_ss.

examples/RSA/binomialScript.sml
@@ -4,17 +4,14 @@ struct
 open HolKernel Parse boolLib bossLib
      arithmeticTheory factorialTheory powerTheory summationTheory ;
 
-infix THEN THENC THENL;
-infix 8 by;
-
 val ARW = RW_TAC arith_ss;
 
 val _ = new_theory "binomial";
 
 
-val BINOMIAL = 
- Define 
-     `(binomial a 0  = 1) 
+val BINOMIAL =
+ Define
+     `(binomial a 0  = 1)
   /\  (binomial 0 (SUC b) = 0)
   /\  (binomial (SUC a) (SUC b) = binomial a (SUC b) + binomial a b)`;
 
@@ -25,7 +22,7 @@ val BINOMIAL_DEF1 = store_thm("BINOMIAL_DEF1",
 
 val BINOMIAL_DEF2 = store_thm("BINOMIAL_DEF2",
 			Term `!a b. a < b ==> (binomial a b = 0)`,
-                        Induct_on `a` THEN Cases_on `b` 
+                        Induct_on `a` THEN Cases_on `b`
                         THEN REWRITE_TAC[BINOMIAL] THEN ARW[]);
 
 val BINOMIAL_DEF3 = store_thm("BINOMIAL_DEF3",
@@ -34,19 +31,19 @@ val BINOMIAL_DEF3 = store_thm("BINOMIAL_DEF3",
                         THEN ARW[BINOMIAL_DEF2]);
 
 val BINOMIAL_DEF4 = store_thm("BINOMIAL_DEF4",
-			Term `!a b. binomial (SUC a) (SUC b) 
-                                       = 
+			Term `!a b. binomial (SUC a) (SUC b)
+                                       =
                                     binomial a (SUC b) + binomial a b`,
                         REWRITE_TAC[BINOMIAL]);
 
 val BINOMIAL_FACT = store_thm("BINOMIAL_FACT",
-Term `!a b. binomial (a+b) b * (fact a * fact b) 
-              = 
+Term `!a b. binomial (a+b) b * (fact a * fact b)
+              =
             fact (a+b)`,
 Induct_on `b`
   THENL [
     REWRITE_TAC[BINOMIAL_DEF1,fact_def,ADD_CLAUSES,MULT_CLAUSES],
-    Induct_on `a` 
+    Induct_on `a`
       THENL [
         REWRITE_TAC[BINOMIAL_DEF3,fact_def,ADD_CLAUSES,MULT_CLAUSES],
         `SUC a + SUC b = SUC (SUC a + b)` by ARW[ADD_CLAUSES]
@@ -54,15 +51,15 @@ Induct_on `b`
              THEN `binomial (SUC a + b) (SUC b) * (fact (SUC a) * fact (SUC b))
                     =
                    (binomial (a + SUC b) (SUC b) * (fact a * fact (SUC b)))
-                   * SUC a` 
+                   * SUC a`
                by REWRITE_TAC[fact_def,ADD_CLAUSES]
              THENL [
                PROVE_TAC[MULT_ASSOC,MULT_SYM],
-               ASM_REWRITE_TAC[] 
+               ASM_REWRITE_TAC[]
                  THEN `binomial (SUC a + b) b * (fact (SUC a) * fact (SUC b))
                          =
                        (binomial (SUC a + b) b * (fact (SUC a) * fact b))
-                        * SUC b` 
+                        * SUC b`
                    by REWRITE_TAC[fact_def,ADD_CLAUSES]
                  THENL [
                    PROVE_TAC[MULT_ASSOC,MULT_SYM],
@@ -74,21 +71,21 @@ Induct_on `b`
   ]
 );
 
-
+val power_def' = CONV_RULE numLib.SUC_TO_NUMERAL_DEFN_CONV power_def
 val EXP_PASCAL = store_thm("EXP_PASCAL",
-Term `!a b n. 
-        power (a+b) n 
-          = 
-        summation n 0 
+Term `!a b n.
+        power (a+b) n
+          =
+        summation n 0
           (\k. binomial n k * (power a (n-k) * power b k))`,
-Induct_on `n` 
+Induct_on `n`
  THENL [
   ARW[power_def,summation_def,BINOMIAL_DEF1],
   Cases_on `n`
    THENL [
-     ARW [power_def,summation_def,BINOMIAL_DEF1,BINOMIAL_DEF3,MULT_CLAUSES] 
-       THEN REWRITE_TAC[power_def,ONE,MULT_CLAUSES,ADD_CLAUSES],
-     ONCE_REWRITE_TAC[power_def] 
+     ARW [power_def,summation_def,BINOMIAL_DEF1,BINOMIAL_DEF3,MULT_CLAUSES,
+          power_def'],
+     ONCE_REWRITE_TAC[power_def]
        THEN ASM_REWRITE_TAC[RIGHT_ADD_DISTRIB,SUMMATION_TIMES]
        THEN REPEAT STRIP_TAC
        THEN `summation (SUC n') 0
@@ -97,46 +94,48 @@ Induct_on `n`
              a * power a (SUC n') +
              summation n' 1
                (\n. a * (binomial(SUC n') n * (power a (SUC n' - n) * power b n)))`
-         by ARW[SUMMATION_1,BINOMIAL_DEF1,power_def,MULT_CLAUSES,ONE]
-       THEN `summation (SUC n') 0  
+         by ARW[SUMMATION_1,BINOMIAL_DEF1,power_def',MULT_CLAUSES]
+       THEN `summation (SUC n') 0
               (\n. b * (binomial(SUC n') n * (power a (SUC n' - n) * power b n)))
                =
-             summation n' 0  
+             summation n' 0
                (\n. b * (binomial(SUC n') n * (power a (SUC n' - n) * power b n)))
                + b * power b (SUC n')`
          by ARW [SUMMATION_2,BINOMIAL_DEF1,
-                 BINOMIAL_DEF3,power_def,MULT_CLAUSES,ONE]
+                 BINOMIAL_DEF3,power_def',MULT_CLAUSES]
        THEN BETA_TAC THEN ASM_REWRITE_TAC[]
        THEN REWRITE_TAC[Q.SPECL[`n'`,`0`] SUMMATION_SHIFT] THEN BETA_TAC
-       THEN `(a * power a (SUC n') 
-             + (summation n' 1 
+       THEN `(a * power a (SUC n')
+             + (summation n' 1
                  (\n. a * (binomial(SUC n') n * (power a (SUC n' - n) * power b n)))
              + (summation n' (SUC 0)
                  (\n. b * (binomial(SUC n') (n-1) * (power a (SUC n' - (n-1)) * power b (n-1))))
              + b * power b (SUC n'))))
           =
-             (a * power a (SUC n') 
-             + (summation n' 1 
+             (a * power a (SUC n')
+             + (summation n' 1
                  (\n. binomial (SUC (SUC n')) n * (power a (SUC (SUC n') - n) * power b n))
              + b * power b (SUC n')))` by ALL_TAC
        THENL [
-        ARW [ONE,SUMMATION_ADD]
-          THEN MATCH_MP_TAC SUMMATION_EXT 
-          THEN ARW[ADD_CLAUSES,Q.SPEC`SUC n'` BINOMIAL_DEF4,RIGHT_ADD_DISTRIB]
-          THEN POP_ASSUM MP_TAC THEN REPEAT (POP_ASSUM (K ALL_TAC)) 
+        ASM_SIMP_TAC bool_ss [ONE,SUMMATION_ADD] THEN ARW[SUMMATION_ADD]
+          THEN MATCH_MP_TAC SUMMATION_EXT
+          THEN ARW[ADD_CLAUSES,Q.SPEC`SUC n'` BINOMIAL_DEF4,RIGHT_ADD_DISTRIB,
+                   GSYM ADD1]
+          THEN POP_ASSUM MP_TAC THEN REPEAT (POP_ASSUM (K ALL_TAC))
           THEN DISCH_TAC
           THEN `SUC n' - k = SUC (n' - k)` by ARW[]
-          THEN ASM_REWRITE_TAC[power_def] 
+          THEN ASM_REWRITE_TAC[power_def]
           THEN MATCH_MP_TAC (DECIDE ``(x=q) /\ (y=p) ==> (x + y = p + q)``)
           THEN PROVE_TAC [MULT_SYM,MULT_ASSOC],
-         ASM_REWRITE_TAC [GSYM ADD_ASSOC]
-          THEN ARW[Q.SPEC`SUC n'` SUMMATION_1, Q.SPEC`n'` SUMMATION_2]
+         ASM_REWRITE_TAC [GSYM ADD_ASSOC, ONE]
+          THEN ARW[Q.SPEC`SUC n'` SUMMATION_1, Q.SPEC`n'` SUMMATION_2,
+                   DECIDE ``x + 2 = SUC (SUC x)``]
           THEN ARW[power_def,BINOMIAL_DEF1,MULT_CLAUSES,ADD_CLAUSES]
           THEN ARW[power_def,BINOMIAL_DEF3,MULT_CLAUSES]
+          THEN REWRITE_TAC [TWO]
           THEN ONCE_REWRITE_TAC[SUMMATION_SHIFT_P] THEN BETA_TAC
-          THEN REWRITE_TAC[ONE]
-          THEN MATCH_MP_TAC SUMMATION_EXT 
-          THEN ARW[ADD_SUB]
+          THEN MATCH_MP_TAC SUMMATION_EXT
+          THEN ARW[]
        ]
    ]
  ]);
